Changed core unrestriction and substitution operators to be overloadable, to support Isabelle/UTP integration. Added some extra laws for alphabet lifting.

Extension.thy
@@ -4,31 +4,26 @@ theory Extension
   imports Substitutions
 begin
 
-definition saext :: "('s\<^sub>1 \<Longrightarrow> 's\<^sub>2) \<Rightarrow> ('s\<^sub>2, 's\<^sub>1) psubst" ("_\<^sup>\<up>") where
-[expr_defs]: "saext a = get\<^bsub>a\<^esub>"
+syntax 
+  "_aext"      :: "logic \<Rightarrow> svid \<Rightarrow> logic" (infixl "\<up>" 80)
+  "_ares"      :: "logic \<Rightarrow> svid \<Rightarrow> logic" (infixl "\<down>" 80)
+  "_pre"       :: "logic \<Rightarrow> logic" ("_\<^sup><" [999] 1000)
+  "_post"      :: "logic \<Rightarrow> logic" ("_\<^sup>>" [999] 1000)
+  "_drop_pre"  :: "logic \<Rightarrow> logic" ("_\<^sub><" [999] 1000)
+  "_drop_post" :: "logic \<Rightarrow> logic" ("_\<^sub>>" [999] 1000)
 
-definition sares :: "('s\<^sub>1 \<Longrightarrow> 's\<^sub>2) \<Rightarrow> ('s\<^sub>1, 's\<^sub>2) psubst" ("_\<^sub>\<down>") where
-[expr_defs]: "sares a = create\<^bsub>a\<^esub>"
-
-abbreviation "aext P a \<equiv> subst_app (saext a) P"
-abbreviation "ares P a \<equiv> subst_app (sares a) P"
+translations
+  "_aext P a" == "CONST aext P a"
+  "_ares P a" == "CONST ares P a"
+  "_pre P" == "_aext (P)\<^sub>e fst\<^sub>L"
+  "_post P" == "_aext (P)\<^sub>e snd\<^sub>L"
+  "_drop_pre P" == "_ares (P)\<^sub>e fst\<^sub>L"
+  "_drop_post P" == "_ares (P)\<^sub>e snd\<^sub>L"
 
 expr_ctr aext
 expr_ctr ares
 
-syntax 
-  "_aext" :: "logic \<Rightarrow> svid \<Rightarrow> logic" (infixl "\<up>" 80)
-  "_ares" :: "logic \<Rightarrow> svid \<Rightarrow> logic" (infixl "\<down>" 80)
-  "_pre"  :: "logic \<Rightarrow> logic" ("_\<^sup><" [999] 1000)
-  "_post" :: "logic \<Rightarrow> logic" ("_\<^sup>>" [999] 1000)
-
-translations
-  "_aext P a" == "CONST aext (P)\<^sub>e a"
-  "_ares P a" == "CONST ares (P)\<^sub>e a"
-  "_pre P" == "_aext P fst\<^sub>L"
-  "_post P" == "_aext P snd\<^sub>L"
-
-lemma aext_var: "$x \<up> a = ($a:x)\<^sub>e"
+lemma aext_var: "($x)\<^sub>e \<up> a = ($a:x)\<^sub>e"
   by (simp add: expr_defs lens_defs)
 
 lemma ares_aext: "weak_lens a \<Longrightarrow> P \<up> a \<down> a = P"
@@ -39,9 +34,12 @@ lemma aext_ares: "\<lbrakk> mwb_lens a; (- $a) \<sharp> P \<rbrakk> \<Longrighta
   by (auto simp add: expr_defs fun_eq_iff lens_create_def)
 
 lemma expr_pre [simp]: "e\<^sup>< (s\<^sub>1, s\<^sub>2) = (e)\<^sub>e s\<^sub>1"
-  by (simp add: saext_def subst_app_def)
+  by (simp add: subst_aext_def subst_app_expr_def)
 
 lemma expr_post [simp]: "e\<^sup>> (s\<^sub>1, s\<^sub>2) = (@e)\<^sub>e s\<^sub>2"
-  by (simp add: saext_def subst_app_def)
+  by (simp add: subst_aext_def subst_app_expr_def)
+
+lemma unrest_aext_expr_lens [unrest]: "\<lbrakk> mwb_lens x; x \<bowtie> a \<rbrakk> \<Longrightarrow> $x \<sharp> (P \<up> a)"
+  by (expr_simp add: lens_indep.lens_put_irr2)
 
 end
