Unrestriction.thy
@@ -8,14 +8,18 @@ text \<open> Unrestriction means that an expression does not depend on the value
   described by the given scene (i.e. set of variables) for its valuation. It is a semantic
   characterisation of fresh variables. \<close>
 
-definition unrest :: "'s scene \<Rightarrow> ('b, 's) expr \<Rightarrow> bool" where
-[expr_defs]: "unrest a e = (\<forall> s s'. e (s \<oplus>\<^sub>S s' on a) = e s)"
+consts unrest :: "'s scene \<Rightarrow> 'p \<Rightarrow> bool"
+
+definition unrest_expr :: "'s scene \<Rightarrow> ('b, 's) expr \<Rightarrow> bool" where
+[expr_defs]: "unrest_expr a e = (\<forall> s s'. e (s \<oplus>\<^sub>S s' on a) = e s)"
+
+adhoc_overloading unrest unrest_expr
 
 syntax
   "_unrest" :: "salpha \<Rightarrow> logic \<Rightarrow> logic \<Rightarrow> logic" (infix "\<sharp>" 20)
 
 translations
-  "_unrest x p" == "CONST unrest x (p)\<^sub>e"                                           
+  "_unrest x p" == "CONST unrest x p"                                           
 
 named_theorems unrest
 
@@ -30,65 +34,71 @@ lemma unrest_var_union [unrest]:
 lemma unrest_neg_union:
   assumes "A ##\<^sub>S B" "- A \<sharp> P" "- B \<sharp> P"
   shows "(- (A ; B)) \<sharp> P"
-  using assms by (simp add: unrest_def scene_override_commute scene_override_union)
+  using assms by (simp add: unrest_expr_def scene_override_commute scene_override_union)
 
-lemma unrest_lens:
+text \<open> The following two laws greatly simplify proof when reasoning about unrestricted lens,
+  and so we add them to the expression simplification set. \<close>
+
+lemma unrest_lens [expr_simps]:
   "mwb_lens x \<Longrightarrow> ($x \<sharp> e) = (\<forall> s v. e (put\<^bsub>x\<^esub> s v) = e s)"
-  by (simp add: unrest_def var_alpha_def lens_scene_override comp_mwb_lens lens_override_def)
+  by (simp add: unrest_expr_def var_alpha_def comp_mwb_lens lens_override_def)
      (metis mwb_lens.put_put)
 
-lemma unrest_compl_lens:
+lemma unrest_compl_lens [expr_simps]:
   "mwb_lens x \<Longrightarrow> (- $x \<sharp> e) = (\<forall>s s'. e (put\<^bsub>x\<^esub> s' (get\<^bsub>x\<^esub> s)) = e s)"
-  by (simp add: unrest_def var_alpha_def lens_scene_override comp_mwb_lens lens_override_def scene_override_commute)
+  by (simp add: unrest_expr_def var_alpha_def comp_mwb_lens lens_override_def scene_override_commute)
 
 lemma unrest_subscene: "\<lbrakk> idem_scene a; a \<sharp> e; b \<subseteq>\<^sub>S a \<rbrakk> \<Longrightarrow> b \<sharp> e"
-  by (metis (mono_tags, hide_lams) subscene_eliminate unrest_def)
+  by (metis (mono_tags, hide_lams) subscene_eliminate unrest_expr_def)
 
 lemma unrest_lens_comp [unrest]: "\<lbrakk> mwb_lens x; mwb_lens y; $x \<sharp> e \<rbrakk> \<Longrightarrow> $x:y \<sharp> e"
   by (simp add: unrest_lens, simp add: lens_comp_def ns_alpha_def)
 
-lemma unrest_lit [unrest]: "x \<sharp> \<guillemotleft>v\<guillemotright>"
+lemma unrest_expr [unrest]: "x \<sharp> e \<Longrightarrow> x \<sharp> (e)\<^sub>e"
+  by (simp add: expr_defs)
+
+lemma unrest_lit [unrest]: "x \<sharp> (\<guillemotleft>v\<guillemotright>)\<^sub>e"
   by (simp add: expr_defs)
 
 lemma unrest_var [unrest]: 
-  "\<lbrakk> vwb_lens x; idem_scene a; var_alpha x \<bowtie>\<^sub>S a \<rbrakk> \<Longrightarrow> a \<sharp> $x"
-  by (auto simp add: unrest_def scene_indep_override var_alpha_def)
-     (metis lens_override_def lens_override_idem lens_scene_override mwb_lens_weak vwb_lens_mwb weak_lens_def)
+  "\<lbrakk> vwb_lens x; idem_scene a; var_alpha x \<bowtie>\<^sub>S a \<rbrakk> \<Longrightarrow> a \<sharp> ($x)\<^sub>e"
+  by (auto simp add: unrest_expr_def scene_indep_override var_alpha_def)
+     (metis lens_override_def lens_override_idem mwb_lens_weak vwb_lens_mwb weak_lens_def)
 
 lemma unrest_var': 
-  "x \<notin>\<^sub>S a \<Longrightarrow> a \<sharp> $x"
-  by (simp add: unrest_def)
+  "x \<notin>\<^sub>S a \<Longrightarrow> a \<sharp> ($x)\<^sub>e"
+  by (simp add: unrest_expr_def)
 
 lemma unrest_var_single [unrest]:
-  "\<lbrakk> mwb_lens x; x \<bowtie> y \<rbrakk> \<Longrightarrow> $x \<sharp> $y"
-  by (simp add: expr_defs lens_indep.lens_put_irr2 lens_indep_sym lens_override_def lens_scene_override var_alpha_def)
+  "\<lbrakk> mwb_lens x; x \<bowtie> y \<rbrakk> \<Longrightarrow> $x \<sharp> ($y)\<^sub>e"
+  by (simp add: expr_defs lens_indep.lens_put_irr2 lens_indep_sym lens_override_def var_alpha_def)
 
 lemma unrest_conj [unrest]:
-  "\<lbrakk> x \<sharp> P; x \<sharp> Q \<rbrakk> \<Longrightarrow> x \<sharp> (P \<and> Q)"
+  "\<lbrakk> x \<sharp> P; x \<sharp> Q \<rbrakk> \<Longrightarrow> x \<sharp> (P \<and> Q)\<^sub>e"
   by (auto simp add: expr_defs)
 
 lemma unrest_not [unrest]:
-  "\<lbrakk> x \<sharp> P \<rbrakk> \<Longrightarrow> x \<sharp> (\<not> P)"
+  "\<lbrakk> x \<sharp> P \<rbrakk> \<Longrightarrow> x \<sharp> (\<not> P)\<^sub>e"
   by (auto simp add: expr_defs)
 
 lemma unrest_disj [unrest]:
-  "\<lbrakk> x \<sharp> P; x \<sharp> Q \<rbrakk> \<Longrightarrow> x \<sharp> (P \<or> Q)"
+  "\<lbrakk> x \<sharp> P; x \<sharp> Q \<rbrakk> \<Longrightarrow> x \<sharp> (P \<or> Q)\<^sub>e"
   by (auto simp add: expr_defs)
 
 lemma unrest_implies [unrest]:
-  "\<lbrakk> x \<sharp> P; x \<sharp> Q \<rbrakk> \<Longrightarrow> x \<sharp> (P \<longrightarrow> Q)"
+  "\<lbrakk> x \<sharp> P; x \<sharp> Q \<rbrakk> \<Longrightarrow> x \<sharp> (P \<longrightarrow> Q)\<^sub>e"
   by (auto simp add: expr_defs)
 
 lemma unrest_uop:
-  "\<lbrakk> x \<sharp> e \<rbrakk> \<Longrightarrow> x \<sharp> \<guillemotleft>f\<guillemotright> e"
+  "\<lbrakk> x \<sharp> e \<rbrakk> \<Longrightarrow> x \<sharp> (\<guillemotleft>f\<guillemotright> e)\<^sub>e"
   by (auto simp add: expr_defs)
 
 lemma unrest_bop:
-  "\<lbrakk> x \<sharp> e\<^sub>1; x \<sharp> e\<^sub>2 \<rbrakk> \<Longrightarrow> x \<sharp> \<guillemotleft>f\<guillemotright> e\<^sub>1 e\<^sub>2"
+  "\<lbrakk> x \<sharp> e\<^sub>1; x \<sharp> e\<^sub>2 \<rbrakk> \<Longrightarrow> x \<sharp> (\<guillemotleft>f\<guillemotright> e\<^sub>1 e\<^sub>2)\<^sub>e"
   by (auto simp add: expr_defs)
 
 lemma unrest_trop:
-  "\<lbrakk> x \<sharp> e\<^sub>1; x \<sharp> e\<^sub>2; x \<sharp> e\<^sub>3 \<rbrakk> \<Longrightarrow> x \<sharp> \<guillemotleft>f\<guillemotright> e\<^sub>1 e\<^sub>2 e\<^sub>3"
+  "\<lbrakk> x \<sharp> e\<^sub>1; x \<sharp> e\<^sub>2; x \<sharp> e\<^sub>3 \<rbrakk> \<Longrightarrow> x \<sharp> (\<guillemotleft>f\<guillemotright> e\<^sub>1 e\<^sub>2 e\<^sub>3)\<^sub>e"
   by (auto simp add: expr_defs)
 
 end
